coq/ExtendedValidation.v
@@ -112,9 +112,9 @@ Hint Constructors valid_values.
 Reserved Notation " '⊢r' r ∈ ts" (at level 70).
 Inductive valid_result : result -> list valtype -> Prop :=
 
-  | VR_val : forall vals ts,
+  | VR_vals : forall vals ts,
       Forall2 (fun val t => ⊢v val ∈ t) vals ts ->
-      ⊢r R_val vals ∈ ts
+      ⊢r R_vals vals ∈ ts
 
   | VR_trap : forall ts,
       ⊢r R_trap ∈ ts
@@ -248,6 +248,26 @@ Inductive valid_tableinst : store -> tableinst -> tabletype -> Prop :=
 where "S '⊢ti' ti '∈' tt"  := (valid_tableinst S ti tt).
 Hint Constructors valid_tableinst.
 
+Definition gen_tabletype (ti: tableinst) : tabletype :=
+  let n := length ti.(TI_elem) in
+  let m__opt := ti.(TI_max) in
+  ({| L_min := n; L_max := m__opt  |}, funcref).
+
+Lemma valid_gen_tabletype : forall S tableinst,
+    S ⊢ti tableinst ∈ gen_tabletype(tableinst).
+Proof with auto.
+  intros.
+  destruct tableinst.
+  unfold gen_tabletype. simpl.
+  constructor...
+  constructor.
+  destruct TI_max.
+  - apply VL__some. 
+    + (* need all I32.t less than I32.max *) skip.
+    + skip.
+    + skip.
+  - apply VL__none. admit.
+Admitted.
 
 (** This is not explicitly defined but occured as
 
@@ -263,6 +283,18 @@ Inductive valid_tableinsts : store -> list tableinst -> list tabletype -> Prop :
 where "S '⊢ti*' tis ∈ tts" := (valid_tableinsts S tis tts).
 Hint Constructors valid_tableinsts.
 
+Definition gen_tabletypes (tis: list tableinst) : list tabletype :=
+  map gen_tabletype tis.
+
+Lemma valid_gen_tabletypes : forall S tableinsts,
+    S ⊢ti* tableinsts ∈ gen_tabletypes(tableinsts).
+Proof.
+  intros.
+  constructor.
+  induction tableinsts; constructor.
+  - apply valid_gen_tabletype.
+  - apply IHtableinsts.
+Qed.
 
 (* ----------------------------------------------------------------- *)
 (** *** Store *)
@@ -284,7 +316,6 @@ Inductive valid_store : store -> Prop :=
 
 where "'⊢S' S 'ok' " := (valid_store S).
 Hint Constructors valid_store.
-
 
 
 (* ================================================================= *)
@@ -349,8 +380,8 @@ with valid_admin_instr : (store * context) -> admin_instr -> functype -> Prop :=
       C ⊢ instr ∈ ft ->
       (S,C) ⊢a (instr: admin_instr) ∈ ft
 
-  (* | VAI_trap : forall S C ts1 ts2, *)
-  (*     (S,C) ⊢a Trap ∈ ts1 --> ts2 *)
+  | VAI_trap : forall S C ts1 ts2,
+      (S,C) ⊢a Trap ∈ ts1 --> ts2
 
   (* | VAI_invoke : forall S C fa ts1 ts2, *)
   (*     (* TODO: external check *)
@@ -375,10 +406,22 @@ with valid_admin_instr : (store * context) -> admin_instr -> functype -> Prop :=
 
 with valid_admin_instrs : store * context -> list admin_instr -> functype -> Prop :=
 
-  | VAIS: forall S C (instrs : list instr) ft,
-      C ⊢* instrs ∈ ft ->
-      (S,C) ⊢a* ↑instrs ∈ ft
+(* I was naively doing below but it's obviously wrong. 
 
+    | VAIS: forall S C (instrs : list instr) ft,
+        C ⊢* instrs ∈ ft ->
+        (S,C) ⊢a* ↑instrs ∈ ft
+
+   The possible correct way is to _duplicate_ the [valid_instrs] pattern?
+*)
+
+  | VAIS_empty : forall S C ts,
+      (S,C) ⊢a* [] ∈ ts --> ts
+
+  | VAIS_snoc : forall S C ainstrs ainstr__N ts0 ts1 ts ts3,
+      (S,C) ⊢a* ainstrs ∈ ts1 --> (ts0 ++ ts) (* ts2 *) ->
+      (S,C) ⊢a  ainstr__N ∈ ts --> ts3 ->
+      (S,C) ⊢a* ainstrs ++ [ainstr__N] ∈ ts1 --> (ts0 ++ ts3)
 
 where "S_C '⊢a' ainstr '∈' ft " := (valid_admin_instr S_C ainstr ft)
   and "S_C '⊢a*' ainstrs '∈' ft" := (valid_admin_instrs S_C ainstrs ft)
@@ -483,3 +526,232 @@ Inductive extend_store : store -> store -> Prop :=
 
 where "⊢S S1 '⪯' S2" := (extend_store S1 S2).
 Hint Constructors extend_store.
+
+
+(* ================================================================= *)
+(** ** Lemmas *)
+
+(* Extending funcinsts relation only holds as reflexivity. *)
+Lemma extend_funcinsts_refl: forall fis fis',
+    ⊢fi* fis ⪯ fis' <->
+    fis = fis'.
+Proof with auto.
+  split.
+  - (* -> *) 
+    introv HEFIS.
+    inverts HEFIS as HForall2.
+    induction HForall2; try inverts H; subst...
+  - (* <- *)
+    introv Heq; subst.
+    induction fis'.
+    + constructor; constructor.
+    + constructor. constructor. constructor. inverts IHfis'...
+Qed.
+
+(* Weaker than [extend_funcinst_refl] by only implying [<-] direction *)
+Lemma extend_tableinst_refl: forall ti,
+    ⊢ti ti ⪯ ti. 
+Proof with auto.
+  intros.
+  destruct ti eqn:Heqti.
+  rename TI_elem into elems.
+  remember (length elems) as n.
+  econstructor;
+   try (symmetry; eassumption)...
+Qed.
+
+Lemma extend_tableinsts_refl: forall tis,
+    ⊢ti* tis ⪯ tis. 
+Proof with auto.
+  intros.
+  constructor.
+  induction tis; constructor.
+  - apply extend_tableinst_refl.
+  - apply IHtis.
+Qed.
+
+(* Weakening an appended funcinst list validity to its subset. *)
+Lemma valid_funcinsts_app: forall S funcinsts functypes funcinsts1 funcinsts2,
+  S ⊢fi* funcinsts ∈ functypes ->
+  funcinsts = funcinsts1 ++ funcinsts2 ->
+  exists functypes1 functypes2,
+    S ⊢fi* funcinsts1 ∈ functypes1 /\ S ⊢fi* funcinsts2 ∈ functypes2.
+Proof with auto.
+  introv HVFIS Heq.
+  subst.
+  inverts HVFIS as HForall2.
+  apply Forall2_app_inv_l in HForall2.
+  destruct HForall2 as (ft1 & ft2 & Hft1 & Hft2 & Hfteq).
+  exists ft1 ft2. split; constructor...
+Qed.
+
+(* Weakening an appended tableinst list validity to its subset. *)
+Lemma valid_tableinsts_app: forall S tableinsts tabletypes tableinsts1 tableinsts2,
+  S ⊢ti* tableinsts ∈ tabletypes ->
+  tableinsts = tableinsts1 ++ tableinsts2 ->
+  exists tabletypes1 tabletypes2,
+    S ⊢ti* tableinsts1 ∈ tabletypes1 /\ S ⊢ti* tableinsts2 ∈ tabletypes2.
+Proof with auto.
+  introv HVTIS Heq.
+  subst.
+  inverts HVTIS as HForall2.
+  apply Forall2_app_inv_l in HForall2.
+  destruct HForall2 as (tt1 & tt2 & Htt1 & Htt2 & Htteq).
+  exists tt1 tt2. split; constructor...
+Qed.
+
+
+(* I think the below two lemmas are not stated correct *)
+Lemma valid_tableinst_weakening: forall S tableinst1 tableinst2 tabletype,
+      ⊢ti tableinst1 ⪯ tableinst2 ->
+    S ⊢ti tableinst1 ∈ tabletype ->
+    S ⊢ti tableinst2 ∈ tabletype.
+Proof.
+  introv HETI HVTI1.
+  inverts HETI as Hleq.
+  inverts HVTI1 as HVTT.
+Abort.
+
+
+Lemma valid_tableinsts_weakening: forall S tableinsts1 tableinsts1' tabletypes1,
+    ⊢ti* tableinsts1 ⪯ tableinsts1' ->
+  S ⊢ti* tableinsts1' ∈ tabletypes1 ->
+  S ⊢ti* tableinsts1 ∈ tabletypes1.
+Proof.
+  introv HETIS HVTIS1.
+  inverts HETIS as HForall2_E.
+  inverts HVTIS1 as HForall2_V.
+  constructor.
+  gen tableinsts1. induction HForall2_V;
+       intros; inverts HForall2_E; constructor.
+  - skip. (* rely on the [valid_tableinst_weakening] and doubt the correctness of this theorem. *)
+  - apply IHHForall2_V. apply H4.
+Abort.
+
+(* We haven't completed all module instance validating (typing),
+   They looks like about checking external values/types.
+   So I should this still holds.
+   Why should this hold intuitively? I don't know yet.
+ *)
+Lemma store_weakening_preserve_type_moduleinst: forall S1 S2 mi C,
+    ⊢S S1 ⪯ S2 ->    (* currently not used, might used for typing externals? NOT SURE *)
+    S2 ⊢mi mi ∈ C ->
+    S1 ⊢mi mi ∈ C.
+Proof with eauto.
+  introv HES HVMI2.
+  inverts HVMI2.
+  econstructor... 
+Qed.
+
+Lemma store_weakening_preserve_type_funcinst: forall S1 S2 fi ft,
+    ⊢S S1 ⪯ S2 ->  (* required due to preserve moduleinst but might not used by that? *)
+    S2 ⊢fi fi ∈ ft ->
+    S1 ⊢fi fi ∈ ft.
+Proof.
+  introv HES HVFI2.
+  inverts HVFI2 as HVFT HVMI2 HVF.
+  econstructor.
+  - assumption.
+  - eapply store_weakening_preserve_type_moduleinst; eassumption. 
+  - assumption.
+Qed.
+
+Lemma store_weakening_preserve_type_tableinst: forall S1 S2 ti tt,
+    ⊢S S1 ⪯ S2 ->  (* not required...valid tableinst is store-irrelvant? *)
+    S2 ⊢ti ti ∈ tt ->
+    S1 ⊢ti ti ∈ tt.
+Proof.
+  introv HES HVTI2.
+  inverts HVTI2 as HVTT.
+  remember (length fes) as n; symmetry in Heqn.
+  econstructor; assumption.
+Qed.
+
+Lemma store_weakening_preserve_type_funcinsts: forall S1 S2 fis fts,
+    ⊢S S1 ⪯ S2 ->
+    (* S_funcs S1 = fis -> (* Intuitively we need this but not used in proof *) *)
+    S2 ⊢fi* fis ∈ fts ->
+    S1 ⊢fi* fis ∈ fts.
+Proof.
+  introv HES (* Heqfis *) HVFIS2.
+  constructor.
+  inverts HVFIS2 as HForall2.
+  (* clear Heqfis. (* otherwise, it's induction-irrelvant but occur as premises *) *)
+  induction HForall2; constructor.
+  - eapply store_weakening_preserve_type_funcinst; eassumption.
+  - apply IHHForall2. 
+Qed.
+
+Lemma store_weakening_preserve_type_tableinsts: forall S1 S2 tis tts,
+    ⊢S S1 ⪯ S2 ->
+    (* S_tables S1 = tis -> *)
+    S2 ⊢ti* tis ∈ tts ->
+    S1 ⊢ti* tis ∈ tts.
+Proof.
+  introv HES (* Heqtis *) HVTIS2.
+  constructor.
+  inverts HVTIS2 as HForall2.
+  (* clear Heqtis. *)
+  induction HForall2; constructor.
+  - eapply store_weakening_preserve_type_tableinst; eassumption.
+  - apply IHHForall2.
+Qed.
+
+(* Weakening an extended store validity to its subset, not vice versa *)
+Lemma store_weakening: forall S1 S2,
+    ⊢S S2 ok ->
+    ⊢S S1 ⪯ S2 ->
+    ⊢S S1 ok.
+Proof with auto.
+  introv HSok2 HES.
+  inverts HSok2 as HVFIS2 HVTIS2.
+  inverts keep HES as HFIeq HEFIS1' HTIeq HETIS1'; simpl in *.
+  remember {| S_funcs := funcinsts; S_tables := tableinsts |} as S2.
+  destruct S1. 
+  rename S_funcs into funcinsts1.
+  rename S_tables into tableinsts1.
+  remember {| S_funcs := funcinsts1; S_tables := tableinsts1 |} as S1.
+
+  (* For goal 1,2. Lifted to here because of Coq's bug *)
+  specialize (valid_funcinsts_app _ _ _ _ _ HVFIS2 HFIeq)
+    as (functypes1 & functypes2 & HVFIS21 & HVFIS22).
+  specialize (valid_tableinsts_app _ _ _ _ _ HVTIS2 HTIeq)
+    as (tabletypes1 & tabletypes2 & HVTIS21 & HVTIS22).
+
+  econstructor.
+  - (* S1 VFIS *)
+    apply store_weakening_preserve_type_funcinsts with S2.
+    + assumption.
+    (* + apply extend_funcinsts_refl in HEFIS1'. apply HEFIS1'. *)
+    + apply HVFIS21.
+  - (* S1 VTIS *) 
+    apply store_weakening_preserve_type_tableinsts with S2.
+    + assumption.
+    (* + instantiate (1 := tableinsts1). subst... *)
+    + rewrite -> HeqS1 in HETIS1'. simpl in HETIS1'.
+      instantiate (1 := gen_tabletypes (tableinsts1)).
+      apply valid_gen_tabletypes.
+  - (* S1 contents - this one add "exists" constraints. *)
+    apply extend_funcinsts_refl in HEFIS1'. 
+    subst...
+Qed.
+
+                      
+Lemma extend_store_refl: forall S,
+    ⊢S S ok ->
+    ⊢S S ⪯ S.
+Proof with auto.
+  introv HSok.
+  inverts HSok as HVFIS HVTIS.
+  econstructor; auto.
+  - instantiate (1 := []); instantiate (1 := funcinsts). symmetry; apply app_nil_r...
+  - constructor; simpl.
+    assert (Heq : funcinsts = funcinsts). reflexivity.
+    apply (extend_funcinsts_refl funcinsts funcinsts) in Heq.
+    inverts Heq...
+  - instantiate (1 := []); instantiate (1 := tableinsts). symmetry; apply app_nil_r...
+  - constructor; simpl.
+    specialize (extend_tableinsts_refl tableinsts). intros Heq.
+    inverts Heq...
+Qed.
+
