coq/Preservation.v
@@ -11,11 +11,11 @@ From Wasm Require Export Validation.
 From Wasm Require Export Execution.
 From Wasm Require Export ExtendedValidation.
 
-From Wasm.Lib Require Export LibTactics.
-
-
 (* Coercions are too confusing during proofs. *)
 Set Printing Coercions.
+
+(* Sometimes. *)
+(* Unset Printing Notations. *)
 
 
 (**************************************************************)
@@ -30,7 +30,7 @@ Implicit Type val : val.
 Implicit Type vals : list val.
 
 (* Structure *)
-Implicit Type M: module.
+Implicit Type M : module.
 Implicit Type l : labelidx.
 
 Implicit Type instr : instr.
@@ -55,6 +55,7 @@ Implicit Type C : context.
 
 (* Execution *)
 Implicit Type cfg : config.
+Implicit Type res : result.
 Implicit Type S : store.
 Implicit Type F : frame.
 Implicit Type T : thread.
@@ -76,9 +77,12 @@ Implicit Type tis tableinsts: list tableinst.
 Implicit Type Mi mi moduleinst: moduleinst.
 
 
-
 (* ================================================================= *)
-(** ** List snoc / app - Aux *)
+(** ** List Aux - [snoc] or [snoc-app], a.k.a append-unit-on-tail *)
+
+
+(* ----------------------------------------------------------------- *)
+(** *** Snoc *)
 
 Fixpoint snoc {X: Type} (l: list X) (x: X) : list X :=
   match l with
@@ -86,7 +90,7 @@ Fixpoint snoc {X: Type} (l: list X) (x: X) : list X :=
     | h :: t => h :: (snoc t x)
   end.
 
-Lemma length_snoc: forall {X: Type} (l: list X) (x: X),
+Lemma snoc_length: forall {X: Type} (l: list X) (x: X),
   length (snoc l x) = (length l) + 1.
 Proof.
   intros X l x.
@@ -94,17 +98,6 @@ Proof.
   reflexivity.
   simpl.
   rewrite -> IHl'.
-  reflexivity.
-Qed.
-
-Lemma snoc_eq_app: forall {X: Type} (l: list X) (x: X),
-    snoc l x = l ++ [x].
-Proof.
-  intros X l x.
-  induction l.
-  reflexivity.
-  simpl.
-  rewrite IHl.
   reflexivity.
 Qed.
 
@@ -119,24 +112,204 @@ Proof.
   reflexivity.
 Qed.
 
-Lemma snoc_destruct: forall {X: Type} (l1 l2: list X) (x1 x2: X),
+
+(* ----------------------------------------------------------------- *)
+(** *** Snoc_app, or Snoc-style Append *)
+
+Lemma snoc_eq_snoc_app: forall {X: Type} (l: list X) (x: X),
+    snoc l x = l ++ [x].
+Proof.
+  intros X l x.
+  induction l.
+  reflexivity.
+  simpl.
+  rewrite IHl.
+  reflexivity.
+Qed.
+
+(* It's named [app_inj_tail] in the standard lib [List.v], but it's a little bit
+   misleading in that [tail] usually refers to list, not unit (singleton). e.g.
+
+   Check app_inj_tail.
+   Check app_inv_tail.
+
+ *)
+Lemma snoc_app_inj: forall {X: Type} (l1 l2: list X) (x1 x2: X),
+    l1 ++ [x1] = l2 ++ [x2] <->
+    l1 = l2 /\ x1 = x2.
+Proof.
+  split.
+  - apply app_inj_tail.
+  - intros [H1 H2]. subst. reflexivity.
+Qed.
+
+(* easier to prove via [snoc_app_inj] *)
+Lemma snoc_inj: forall {X: Type} (l1 l2: list X) (x1 x2: X),
     snoc l1 x1 = snoc l2 x2 ->
     l1 = l2 /\ x1 = x2.
-Proof.
-  Admitted.
+Proof with auto.
+  introv H.
+  asserts_rewrite (snoc l1 x1 = l1 ++ [x1]) in H. apply snoc_eq_snoc_app.
+  asserts_rewrite (snoc l2 x2 = l2 ++ [x2]) in H. apply snoc_eq_snoc_app.
+  apply app_inj_tail...
+Qed.
 
-Lemma app_snoc_destruct: forall {X: Type} (l1 l2: list X) (x1 x2: X),
-    l1 ++ [x1] = l2 ++ [x2] ->
-    l1 = l2 /\ x1 = x2.
-Proof.
-  Admitted.
 
-Fixpoint unsnoc {X: Type} (l: list X) : option X :=
+Lemma snoc_app_eq_unit : forall {X: Type} (xs: list X) (x1 x2: X),
+    xs ++ [x1] = [x2] ->
+    xs = [] /\ x1 = x2.
+Proof with auto.
+  introv Heq.
+  apply app_eq_unit in Heq.
+  destruct Heq as [[H1 H2] | [H3 H4]].
+  split...
+  - inverts H2...
+  - inverts H4...
+Qed.
+
+Lemma eq_len_eq : forall {X: Type} (xs1 xs2: list X), 
+    xs1 = xs2 -> length xs1 = length xs2.
+Proof with auto.
+  introv Heq.
+  subst...
+Qed.
+
+Lemma plus_0_n_rev : forall x y,
+    x + y = y -> x = 0.
+Proof. 
+  intros. omega.
+Qed.
+
+Lemma snoc_app_eq_same_len : forall {X: Type} (xs xs1 xs2: list X), 
+    length xs1 = length xs2 ->
+    xs ++ xs1 = xs2 ->
+    xs = [] /\ xs1 = xs2.
+Proof with auto.
+  introv Heqlen Heq.
+  assert (Hnil : xs = []).
+  { apply eq_len_eq in Heq.
+    rewrite app_length in Heq.
+    rewrite Heqlen in Heq.
+    apply plus_0_n_rev in Heq.
+    apply length_zero_iff_nil...
+  }
+  subst...
+Qed.
+        
+
+
+(* ----------------------------------------------------------------- *)
+(** *** Unsnoc, destruct car/cdr by snoc *)
+
+Fixpoint unsnoc {X: Type} (l: list X) : option (list X * X) :=
   match l with
     | [] => None 
-    | [x] => Some x
-    | _ :: xs => (unsnoc xs)
+    | [x] => Some ([], x)
+    | x :: xs =>
+      match (unsnoc xs) with
+        | Some (cdr, car) => Some (x :: cdr, car)
+        | None => None
+      end
   end.
+
+(* Similar with [last] but returning option *)
+Fixpoint unsnoc_car {X: Type} (l: list X) : option X :=
+  match l with
+    | [] => None
+    | [x] => Some x
+    | _ :: xs => (unsnoc_car xs)
+  end.
+
+(* the similar weakening for [unsnoc] need to consider [cdr] part *)
+Lemma unsnoc_car_weaken: forall {X: Type} (xs: list X) (x: X),
+    xs <> [] ->
+    unsnoc_car (x::xs) = unsnoc_car xs.
+Proof.
+  intros.
+  destruct xs.
+  - false H. reflexivity.
+  - remember (x0 :: xs) as xs'.
+    simpl. subst. reflexivity.
+Qed.
+
+Lemma exists_unsnoc: forall {X: Type} (xs : list X), 
+    xs <> [] ->
+    exists xs' x, unsnoc xs = Some (xs', x). 
+Proof with auto.
+  introv Hneq.
+  induction xs.
+  - contradiction Hneq...
+  - destruct xs eqn:Hd.
+    + exists (@nil X) a...
+    + destruct IHxs.
+      ++ intros H. inverts H.
+      ++ destruct H.
+         exists (a::x0) x1.
+         remember (x::l) as xs'.
+         simpl.
+         rewrite Heqxs'.
+         rewrite <- Heqxs'.
+         rewrite H.
+         reflexivity.
+Qed.
+
+(* Similar with [exists_last] *)
+Lemma exists_unsnoc_car: forall {X: Type} (xs : list X), 
+    xs <> [] ->
+    exists x, unsnoc_car xs = Some x.
+Proof with auto.
+  introv Hneq.
+  induction xs.
+  - contradiction Hneq...
+  - destruct xs eqn:Hd.
+    + exists a...
+    + destruct IHxs.
+      ++ intros H. inverts H.
+      ++ exists x0.
+         remember (x::l) as xs'.
+         simpl.
+         rewrite Heqxs'.
+         rewrite <- Heqxs'.
+         rewrite H.
+         reflexivity.
+Qed.
+      
+Lemma unsnoc_car_nil : forall {A : Type} (l : list A), 
+    unsnoc_car l = None ->
+    l = nil.
+Proof. 
+  introv H.
+  destruct l.
+  - reflexivity.
+  - assert (Ha : a :: l <> []).
+    + unfold not. intro Hn. inverts Hn.
+    + apply exists_unsnoc_car in Ha. destruct Ha. 
+      rewrite H in H0. inverts H0.
+Qed.
+
+Lemma eq_unsnoc_eq: forall {A : Type} (l1 l2 : list A), 
+  l1 = l2 ->
+  unsnoc l1 = unsnoc l2.
+Proof with auto. 
+  introv Heq.
+  gen l2. induction l1; destruct l2; intros.
+  - reflexivity.
+  - inverts Heq.
+  - inverts Heq.
+  - injection Heq. intros; subst...
+Qed.
+
+Lemma eq_unsnoc_car_eq: forall {A : Type} (l1 l2 : list A), 
+  l1 = l2 ->
+  unsnoc_car l1 = unsnoc_car l2.
+Proof with auto. 
+  introv Heq.
+  gen l2. induction l1; destruct l2; intros.
+  - reflexivity.
+  - inverts Heq.
+  - inverts Heq.
+  - injection Heq. intros; subst...
+Qed.
 
 Lemma unsnoc_neq: forall {A : Type} (l1 l2 : list A), 
   unsnoc l1 <> unsnoc l2 ->
@@ -144,76 +317,402 @@ Lemma unsnoc_neq: forall {A : Type} (l1 l2 : list A),
 Proof. 
   Admitted.
 
-Lemma unsnoc_snoc_app : forall {X: Type} (l: list X) x,
-    unsnoc (l ++ [x]) = Some x.
+Lemma unsnoc_car_neq: forall {A : Type} (l1 l2 : list A), 
+  unsnoc_car l1 <> unsnoc_car l2 ->
+  l1 <> l2.
 Proof. 
   Admitted.
 
-Lemma unsnoc_snoc : forall {X: Type} (l: list X) x,
-    unsnoc (snoc l x) = Some x.
+Lemma unsnoc_snoc_app_some : forall {X: Type} (l: list X) x,
+    unsnoc (l ++ [x]) = Some (l, x).
 Proof. 
   Admitted.
+
+Lemma unsnoc_some_eq_snoc_app: forall {X: Type} {xs xs' : list X} {x: X},
+  unsnoc xs = Some (xs', x) ->
+  xs = xs' ++ [x].
+Proof with auto.
+  destruct xs;
+    introv Heq.
+  - simpl in Heq. inverts Heq.
+  - gen x xs'. induction xs; intros.
+    + simpl in Heq. inverts Heq. apply app_nil_l.
+    + admit.
+Admitted.
+
+
+Lemma unsnoc_car_snoc_app_some : forall {X: Type} (l: list X) x,
+    unsnoc_car (l ++ [x]) = Some x.
+Proof. 
+  Admitted.
+
+Lemma unsnoc_snoc_some : forall {X: Type} (l: list X) x,
+    unsnoc (snoc l x) = Some (l, x).
+Proof. 
+  Admitted.
+
+Lemma unsnoc_car_snoc_some : forall {X: Type} (l: list X) x,
+    unsnoc_car (snoc l x) = Some x.
+Proof. 
+  Admitted.
+
+(* This give only the existentials but could not take advantages of Coq computing engine. *) 
+Lemma eq_snoc_app_split_exist: forall {X:Type} (ys xs': list X) (x: X),
+    ys = xs' ++ [x] ->
+    exists ys' y,
+      ys = ys' ++ [y] /\ ys' = xs' /\ y = x.
+Proof with auto.
+  introv Heq.
+  destruct ys as [ | y ys'] eqn:Heqys.
+  - (* [] - prove it's impossible *)
+    symmetry in Heq. apply app_eq_nil in Heq.
+    destruct Heq as [H1 Hconstr]. inverts Hconstr.
+  - (* :: then we can construct the existential *)
+    assert (Hneq : ys <> []). { subst. unfold not; intros. inverts H. }
+    destruct (exists_unsnoc ys Hneq) as (cdr & car & Hunsnoc).
+    exists cdr car.
+    split.
+    + subst ys. rewrite -> Heq in *.
+      rewrite unsnoc_snoc_app_some in Hunsnoc.
+      inverts keep Hunsnoc. reflexivity.
+    + (* prove cdr ++ [car] = xs' ++ [x] *)
+      rewrite <- Heqys in Heq.
+      apply eq_unsnoc_eq in Heq. 
+      rewrite -> Hunsnoc in Heq.
+      rewrite unsnoc_snoc_app_some in Heq.
+      splits; injection Heq; auto.
+Qed.
+
+(* By introducing the [Fixpoint unsnoc] we add some computing power for [simpl] to perform. *)
+Lemma eq_snoc_app_split_unsnoc: forall {X:Type} (ys xs': list X) (x: X),
+    ys = xs' ++ [x] ->
+    unsnoc ys = Some (xs', x).
+Proof with auto.
+  introv Heq.
+  apply eq_snoc_app_split_exist in Heq.
+  destruct Heq as (ys' & y & Heq & Hys' & Hy).
+  rewrite -> Heq.
+  asserts_rewrite (unsnoc (ys' ++ [y]) = Some (ys', y)).
+  apply unsnoc_snoc_app_some.
+  subst...
+Qed.
+
+(* Invert when the snoc-append equation does hold,
+   This will perform the Coq computation and subst the generated equality.
+ *)
+Ltac invert_eq_snoc_app_compute Heq :=
+  apply eq_snoc_app_split_unsnoc in Heq;
+  inverts Heq.
+
+
+(* Inverts when the snoc-append equation does not hold
+   This is for discharging cases that are invalid.
+ *)
+Ltac invert_eq_snoc_app_discharge Heq cdr car :=
+    try solve [
+          apply eq_unsnoc_car_eq in Heq;
+          simpl in Heq;
+          rewrite -> (unsnoc_car_snoc_app_some cdr car) in Heq;
+          inverts Heq
+        ].
+
+(* A powerful pack of both discharging and computing *)
+Ltac invert_eq_snoc_app Heq cdr car :=
+  invert_eq_snoc_app_discharge Heq cdr car;
+  invert_eq_snoc_app_compute Heq.
+
+
+Module InvertEqSnocAppTest.
+
+  Lemma discharge : forall cdr,
+      [1; 2] = cdr ++ [3] ->
+      2 = 3.
+  Proof.
+    dup.
+    - introv Heq.
+      invert_eq_snoc_app_discharge Heq cdr 3.
+    - introv Heq.
+      invert_eq_snoc_app Heq cdr 3.
+  Qed.
+
+  Lemma compute : forall cdr,
+      [1; 2] = cdr ++ [2] ->
+      2 = 2.
+  Proof.
+    dup.
+    - introv Heq.
+      invert_eq_snoc_app_compute Heq. reflexivity.
+    - introv Heq.
+      invert_eq_snoc_app Heq cdr 3. reflexivity.
+  Qed.
+
+End InvertEqSnocAppTest.
+
+
+(* This map version gave what we want. *)
+Lemma map_eq_snoc_app_split: forall {X:Type} {Y: Type} (ys : list Y) (xs': list X) (x: X) (f: Y -> X),
+    map f ys = xs' ++ [x] ->
+    exists ys' y,
+      ys = ys' ++ [y] /\ map f ys' = xs' /\ f y = x.
+Proof with auto.
+  introv Heq.
+  destruct ys as [ | y ys'] eqn:Heqys.
+  - (* ys = [] - prove it's impossible *)
+    symmetry in Heq.
+    apply app_eq_nil in Heq.
+    destruct Heq as [H1 Hconstr]. inverts Hconstr.
+  - (* ys <> [] - then we can unsnoc it and instantiate the existentials *)
+    assert (Hneq : ys <> []) by (apply not_eq_sym; subst; apply nil_cons).  
+    destruct (exists_unsnoc ys Hneq) as (cdr & car & Hunsnoc).
+    apply unsnoc_some_eq_snoc_app in Hunsnoc.
+    rewrite <- Heqys in Heq.
+    rewrite -> Hunsnoc in Heq.
+    rewrite map_app in Heq.
+    simpl in Heq.
+    apply snoc_app_inj in Heq.
+
+    exists cdr car.
+    split; try subst; assumption. 
+Qed.
+
+
+Lemma vals_typing_eq: forall S C vals rt, 
+    (S,C) ⊢a* ⇈vals ∈ [] --> rt ->
+    rt = map type_of vals.
+Proof with auto.
+  introv HVAIS.
+  dependent induction HVAIS;
+    rename x into Heq;
+    symmetry in Heq.
+  - (* VAIS_nil *)
+    apply map_eq_nil in Heq.
+    apply map_eq_nil in Heq.
+    subst...
+  - (* VAIS_snoc *)
+    rename H into HVAI__N.
+    apply map_eq_snoc_app_split in Heq.
+    destruct Heq as (instrs & instr__N & Heq & Hinstrs & Hinstr__N).
+    apply map_eq_snoc_app_split in Heq.
+    destruct Heq as (vals' & val__N & Heq & Hvals' & Hval__N).
+
+    rewrite <- Hinstrs in *.
+    rewrite <- Hinstr__N in *.
+    rewrite <- Hvals' in *.
+    rewrite <- Hval__N in *.
+
+    inverts HVAI__N as HVI__N.
+    inverts HVI__N.
+
+    asserts_rewrite (map type_of vals = map type_of vals' ++ [type_of val__N]).
+    + rewrite -> Heq. apply map_app.
+    + apply snoc_app_inj.
+      split...
+      ++ rewrite <- (app_nil_r ts0). 
+         eapply (IHHVAIS S C vals' (ts0 ++ []))...
+Qed.
 
 
 (* ================================================================= *)
-(** ** Lemma - lifting *)
+(** ** Lemma - equality/injectivitiy between lifting *)
 
-Lemma lift_up_eq : forall instrs1 instrs2,
+(* constructors are injective
+   so we don't need to prove Plain and Const is injective... 
+
+   but we need to prove [map] preserve injectivity.
+ *)
+
+Lemma map_inj_inj: forall {X Y: Type} (f: X -> Y) (xs1 xs2: list X),
+    (forall x1 x2, f x1 = f x2 -> x1 = x2) ->
+    map f xs1 = map f xs2 ->
+    xs1 = xs2.
+Proof with auto.
+  introv Hinj Heq.
+  gen xs2. induction xs1; intros.
+  - simpl in Heq. symmetry in Heq. apply map_eq_nil in Heq. subst...
+  - destruct xs2.
+    + inverts Heq.
+    + asserts_rewrite (map f (a :: xs1) = f a :: map f xs1) in Heq. apply map_cons.
+      asserts_rewrite (map f (x :: xs2) = f x :: map f xs2) in Heq. apply map_cons.
+      inverts Heq.
+      apply Hinj in H0.
+      apply IHxs1 in H1.
+      subst...
+Qed.
+
+Lemma up_inj : forall instrs1 instrs2,
     ↑instrs1 = ↑instrs2 ->
      instrs1 =  instrs2.
-Proof.
-  Admitted.
+Proof with eauto.
+  intros.
+  apply (map_inj_inj Plain)...
+  introv Hinj; inverts Hinj...
+Qed.
+    
 
-Lemma lift_upup_eq : forall vals1 vals2,
-    ⇈vals1 = ⇈vals1 ->
+Lemma lift_vals_inj : forall vals1 vals2,
+    lift_vals vals1 = lift_vals vals2 ->
+              vals1 =           vals2.
+Proof with auto.
+  intros.
+  apply (map_inj_inj Const)...
+  introv Hinj. inverts Hinj...
+Qed.
+
+Lemma upup_inj : forall vals1 vals2,
+    ⇈vals1 = ⇈vals2 ->
      vals1 =  vals2.
-Proof.
-  Admitted.
+Proof with auto.
+  intros.
+  remember (map Const vals1) as instrs1.
+  remember (map Const vals2) as instrs2.
+  apply up_inj in H.
+  apply lift_vals_inj; subst...
+Qed.
 
-Lemma lift_vals_eq : forall vals1 vals2,
-    lift_vals vals1 = lift_vals vals1 ->
-    vals1 =  vals2.
-Proof.
-  Admitted.
 
-(* using [Lemma map_app] *)
-
-Lemma lift_up_app : forall instrs1 instrs2,
+Lemma up_app : forall instrs1 instrs2,
   ↑(instrs1 ++ instrs2) = ↑instrs1 ++ ↑instrs2.
 Proof.
-  Admitted.
-
-Lemma lift_upup_app : forall vals1 vals2,
-  ⇈(vals1 ++ vals2) = ⇈vals1 ++ ⇈vals2.
-Proof.
-  Admitted.
+  apply map_app.
+Qed.
 
 Lemma lift_vals_app : forall vals1 vals2,
   lift_vals (vals1 ++ vals2) = lift_vals vals1 ++ lift_vals vals2.
 Proof.
-  Admitted.
+  apply map_app.
+Qed.
 
+Lemma upup_app : forall vals1 vals2,
+  ⇈(vals1 ++ vals2) = ⇈vals1 ++ ⇈vals2.
+Proof.
+  intros.
+  remember (map Const vals1) as instrs1.
+  remember (map Const vals2) as instrs2.
+  remember (map Const (app vals1 vals2)) as instrs_app.
+  asserts_rewrite (instrs_app = instrs1 ++ instrs2).
+  - subst. apply lift_vals_app.
+  - apply up_app.
+Qed.
+
+Lemma upup_cons : forall val vals,
+  ⇈(val :: vals) = Plain (Const val) :: ⇈vals.
+Proof.
+  intros.
+  remember (Const val) as head.
+  remember (map Const vals) as tail.
+  remember (map Const (cons val vals)) as list.
+  asserts_rewrite (list = head :: tail).
+  - subst. apply map_cons.
+  - apply map_cons.
+Qed.
+
+
+Lemma unsnoc_car_vals : forall vals,
+    unsnoc_car (⇈vals) = None \/ exists val, unsnoc_car (⇈vals) = (Some (Plain (Const val))).
+Proof with auto.
+  intros. 
+  induction vals.
+  - left. simpl...
+  - right.
+    assert (H: ⇈(a :: vals) <> []).
+    + unfold not. intros. inverts H.
+    + destruct IHvals.
+      ++ (* None *)
+        apply unsnoc_car_nil in H0.
+        apply map_eq_nil in H0.
+        apply map_eq_nil in H0.
+        subst. 
+        exists a. simpl...
+      ++ (* Some *)
+        destruct vals.
+        +++ (* [a] *) exists a...
+        +++ (* a :: v :: vals *)
+          assert (Ha: unsnoc_car (⇈ (a :: v :: vals)) = unsnoc_car (⇈ (v :: vals))).
+          ++++ apply unsnoc_car_weaken. unfold not; intros Hn; inversion Hn.
+          ++++ destruct H0. exists x. subst...
+Qed.
+      
 
 (* ================================================================= *)
-(** ** Lemma - Aux *)
+(** ** Lemma - Normal Form *)
+
+Definition relation (X: Type) := X -> X -> Prop.
+
+Definition normal_form {X : Type} (R : relation X) (x : X) : Prop :=
+  ~ exists x', R x x'.
+
+Lemma vals_normal_form_step_simple : forall vals,
+    normal_form step_simple (⇈vals).
+Proof.
+  unfold normal_form. introv. intros H.
+  inverts H as. intros ainstrs' HSC.
+  inverts HSC;
+   try (inverts H;
+        apply eq_unsnoc_car_eq in H2;
+        simpl in H2;
+        specialize (unsnoc_car_vals vals);
+        intros [ Hnone | Hsome ];
+        try (rewrite -> Hnone in H2; inverts H2);
+        try (destruct Hsome; rewrite -> H in H2; inverts H2)).
+Qed.
+
+(* 
+
+Not True
+
+Lemma vals_is_normal_form_step : forall S F vals,
+    normal_form step (S, F, ⇈vals).
+Proof with auto.
+  unfold normal_form. introv. intros H.
+  inverts H as. intros ainstrs' HSS.
+  inverts HSS.
+  - (* SS_simple *)
+    apply (vals_is_normal_form_step_simple vals).
+    exists ainstrs'0...
+  - (* SS_E *)
+*)
 
 Lemma plug_E_ϵ : forall E ainstrs, 
-  plug__E E ainstrs = [] ->
-  ainstrs = [].
+    plug__E E ainstrs = [] ->     (* N.B. not vice versa *)
+    ainstrs = [].
 Proof.
-  Admitted.
+  introv H.
+  induction E.
+  - (* E_hole *)
+    simpl in *. assumption.
+  - (* E_seq *)
+    simpl in *. 
+    apply app_eq_nil in H. destruct H.
+    apply app_eq_nil in H0. destruct H0.
+    apply IHE. assumption.
+  - (* E_label *)
+    simpl in *. 
+    inverts H.
+Qed.
 
-(* if the snoc is [val], then all [val] *)
-Lemma snoc_val_is_normal_form2: forall ainstrs val, 
-  ~ exists ainstrs', ainstrs ++ ⇈[val] ↪s ainstrs'.
+(* snoc a [val] should be either ill-formed or, normally, all [val] *)
+Lemma ainstrs_snoc_app_val_normal_form_step_simple: forall ainstrs val, 
+    normal_form step_simple (ainstrs ++ ⇈[val]).
 Proof.
-  Admitted.
+  unfold normal_form. introv. intros H.
+  inverts H as. intros ainstrs' HSC.
+  inverts HSC;
+    try(apply eq_unsnoc_car_eq in H;
+        simpl in H;
+        specialize (unsnoc_car_snoc_app_some ainstrs (Plain (Const val)));
+        intros Hsome;
+        rewrite -> Hsome in H;
+        inverts H).
+Qed.
       
-Lemma snoc_val_is_normal_form: forall instrs val, 
-  ~ exists ainstrs', ↑(instrs ++ [Const val]) ↪s ainstrs'.
+Lemma instrs_snoc_app_val_normal_form_step_simple: forall instrs val, 
+    normal_form step_simple (↑(instrs ++ [Const val])).
 Proof.
-  Admitted.
-
+  intros.
+  specialize (map_app Plain instrs [Const val]). intros.
+  rewrite H.
+  apply ainstrs_snoc_app_val_normal_form_step_simple.
+Qed.
 
 Lemma S_F_ϵ_is_normal_form : forall S F S' F',
   ~ exists ainstrs', (S, F, []) ↪ (S', F', ainstrs').
@@ -235,6 +734,10 @@ Proof with auto.
     apply plug_E_ϵ in HE; subst.
     apply IHHSC...
 Qed.
+
+
+(* ================================================================= *)
+(** ** Lemma - Unproved *)
 
 (* We observed this is too strong and we need
    a specific [C] and [ts1] (via [remember].
@@ -274,6 +777,7 @@ Proof.
   Admitted.
 
 
+(* TODO: rename into [singleton_instr_typing] *)
 Lemma drop_singleton_typing: forall C instr__N ts1 ts2,
     C ⊢* [instr__N] ∈ ts1 --> ts2 ->
     C ⊢ instr__N ∈ ts1 --> ts2.
@@ -281,7 +785,7 @@ Proof.
   introv HVIS.
   inverts HVIS.
   replace ([instr__N]) with ([] ++ [instr__N]) in H.
-  apply app_snoc_destruct in H.
+  apply snoc_app_inj in H.
   inverts H.
   inverts H3. apply functype_inv. assumption.
   apply app_eq_nil in H.
@@ -290,14 +794,30 @@ Proof.
   reflexivity.
 Qed.
   
-(* TODO: prov in Numerics.v
-   for binop, testop, relop as well.
- *)
-Lemma eval_unop_inv : forall op val1 val,
-    eval_unop op val1 = Ok (Some val) ->
-    type_of op = type_of val.
+Lemma singleton_ainstr_typing: forall S C ainstr__N ts1 ts2,
+    (S,C) ⊢a* [ainstr__N] ∈ ts1 --> ts2 ->
+    (S,C) ⊢a  ainstr__N ∈ ts1 --> ts2.
+Admitted.
+
+
+(* In favor of [vals_typing_eq] *)
+Lemma vals_typing: forall S C vals, 
+     (S,C) ⊢a* ⇈vals ∈ [] --> map type_of vals.
 Proof.
-  Admitted.
+  intros.
+  destruct vals as [ | ival ivals' ]. 
+  - constructor.
+  - remember (ival :: ivals') as vals.
+    destruct (exists_unsnoc vals) as (vals' & val & Hunsnoc).
+    { unfold not. intros. subst. inversion H. }
+    specialize (unsnoc_some_eq_snoc_app Hunsnoc). intros Heqvals2. 
+    rewrite -> Heqvals2.
+    rewrite -> upup_app. simpl.
+    asserts_rewrite (map type_of (vals' ++ [val]) =  map type_of vals' ++ [type_of val]);
+      try apply map_app.
+    apply VAIS_snoc with (ts := []). 
+    + (* We can't prove it because [snoc] is not defined as an inductive relation *)
+Admitted.    
 
 
 (* ================================================================= *)
@@ -306,7 +826,163 @@ Proof.
 
 
 (* ================================================================= *)
+(** ** Preservation - VAIS_snoc -> SC_simple*)
+
+
+Lemma preservation_SC_simple : forall C S ainstrs ainstr__N ainstrs' ts0 ts2 ts3,
+      (S,C) ⊢a* ainstrs ∈ [] --> (ts0 ++ ts2)  -> (* [HVAIS] *)
+      (S,C) ⊢a  ainstr__N ∈ ts2 --> ts3 ->          (* [HVAI__N] *)
+      ainstrs ++ [ainstr__N] ↪s ainstrs' ->        (* [HSS] *)
+(* -------------------------------------------------------------- *)
+      (S,C) ⊢a* ainstrs' ∈ [] --> (ts0 ++ ts3).
+Proof with eauto.
+  introv HVAIS HVAI__N HSS.
+  inverts HVAI__N as.
+
+  - (* VAI_instr *)
+    intros HVI__N.
+    inverts HVI__N.
+
+    + (* VI_const *)
+      exfalso.
+      simpl in HSS.
+      apply (ainstrs_snoc_app_val_normal_form_step_simple ainstrs val).
+      exists ainstrs'...
+
+    + (* VI_unop *)
+      inverts keep HSS as Heval Heq; 
+        invert_eq_snoc_app Heq ainstrs (Plain (Unop op)).
+
+      ++ (* [SS_unop__some] *)
+        rewrite <- (app_nil_l (↑[Const val])).
+        apply VAIS_snoc with (ts := []). 
+
+        +++ (* [] *)
+          specialize (vals_typing_eq S C [val1] _ HVAIS) as Heq; simpl in Heq.
+          destruct (snoc_app_eq_unit _ _ _ Heq) as (Htype_of & Heqts0).
+          subst. constructor.
+
+        +++ (* ↑[Const val] *)
+          apply VAI_instr.
+          apply VI_const.
+          apply eval_unop_preserve_type in Heval...
+
+      ++ (* [SS_unop__none] *)
+        rewrite <- (app_nil_l ([Trap])).
+        apply VAIS_snoc with (ts := []). 
+
+        +++ (* [] *)
+          specialize (vals_typing_eq S C [val1] _ HVAIS) as Heq; simpl in Heq.
+          destruct (snoc_app_eq_unit _ _ _ Heq) as (Htype_of & Heqts0).
+          subst. constructor.
+
+        +++ (* [Trap] *)
+          apply VAI_trap.
+
+
+    + (* VI_binop *)
+      inverts keep HSS as Heval Heq; 
+        invert_eq_snoc_app Heq ainstrs (Plain (Binop op)).
+
+      ++ (* [SS_binop__some] *)
+        rewrite <- (app_nil_l (↑[Const val])).
+        apply VAIS_snoc with (ts := []).
+
+        +++ (* [] *)
+          specialize (vals_typing_eq S C [val1; val2] _ HVAIS) as Heq; simpl in Heq.
+          destruct (snoc_app_eq_same_len ts0 [type_of op; type_of op] [type_of val1; type_of val2])... 
+          subst. constructor.
+
+        +++ (* ↑[Const val] *)
+          apply VAI_instr.
+          apply VI_const.
+          apply eval_binop_preserve_type in Heval...
+
+      ++ (* [SS_binop__none] *)
+        rewrite <- (app_nil_l ([Trap])).
+        apply VAIS_snoc with (ts := []). (* We know [ts] from [Const val]*)
+
+        +++ (* [] *)
+          specialize (vals_typing_eq S C [val1; val2] _ HVAIS) as Heq; simpl in Heq.
+          destruct (snoc_app_eq_same_len ts0 [type_of op; type_of op] [type_of val1; type_of val2])... 
+          subst. constructor.
+
+        +++ (* [Trap] *)
+          apply VAI_trap.
+
+    + (* VI_testop *)
+      inverts keep HSS as Heval Heq; 
+        invert_eq_snoc_app Heq ainstrs (Plain (Testop op)).
+
+      ++ (* [SS_testop] *)
+        rewrite <- (app_nil_l (↑[Const b])).
+        apply VAIS_snoc with (ts := []).
+
+        +++ (* [] *)
+          specialize (vals_typing_eq S C [val1] _ HVAIS) as Heq; simpl in Heq.
+          destruct (snoc_app_eq_unit _ _ _ Heq)... 
+          subst. constructor.
+
+        +++ (* ↑[Const b] *)
+          apply VAI_instr.
+          apply VI_const.
+          simpl... 
+
+    + (* VI_relop *)
+      inverts keep HSS as Heval Heq; 
+        invert_eq_snoc_app Heq ainstrs (Plain (Relop op)).
+
+      ++ (* [SS_testop] *)
+        rewrite <- (app_nil_l (↑[Const b])).
+        apply VAIS_snoc with (ts := []).
+
+        +++ (* [] *)
+          specialize (vals_typing_eq S C [val1; val2] _ HVAIS) as Heq; simpl in Heq.
+          destruct (snoc_app_eq_same_len ts0 [type_of op; type_of op] [type_of val1; type_of val2])... 
+          subst. constructor.
+
+        +++ (* ↑[Const b] *)
+          apply VAI_instr.
+          apply VI_const.
+          simpl... (* ??? *) (* apply eval_relop_preserve_type in Heval... *)
+
+  - (* VAI_trap *)
+    (* Trap can't take a simple step, so all discharged *)
+    inverts keep HSS as Heval Heq; 
+    invert_eq_snoc_app Heq ainstrs (Trap).
+
+Qed.
+
+
+(* Playing with the SC_E proof *)
+(*
+Theorem preservation : forall S T S' T',
+    $(S, T) ↪ $(S', T') ->
+    forall rt, ⊢c (S, T) ∈ rt ->
+    ⊢c (S', T') ∈ rt /\ ⊢S S ⪯ S'.
+Proof with eauto.
+  introv HSC.
+  destruct T as [F ainstrs].
+  destruct T' as [F' ainstrs'].
+  simpl in HSC.
+  remember (S, F, ainstrs) as SF.
+  remember (S', F', ainstrs') as SF'.
+  gen HeqSF HeqSF'.
+  induction HSC.
+  - admit.
+  -
+*)
+
+(* ================================================================= *)
 (** ** Main Theorem *)
+
+(** Instead of using [remember] to keep infomation from getting lost.
+
+    [dependent induction] (from [Coq.Program.Equality]) or
+    [inductions] (from [LibTactics.v]) are used.
+
+    Though w/o [as] the naming is much worse.
+*)
 
 Theorem preservation : forall S T S' T' rt,
     ⊢c (S, T) ∈ rt ->
@@ -314,104 +990,54 @@ Theorem preservation : forall S T S' T' rt,
     ⊢c (S', T') ∈ rt /\ ⊢S S ⪯ S'.
 Proof with eauto.
   introv HVC.
-  gen S' T'.
-  (* valid_config *) inverts HVC as HSok HVT.
-  (* valid_thread *) inverts HVT as HVA HVAIS. 
-     (* valid_frame *) inverts keep HVA as HVMI HVV.  
-     (* valid_admin_instrs *) inverts HVAIS as HVIS.    
 
-  (* Induction on typing derivation of valid_instrs have 2 cases.
-     We need to remember all specifics otherwise they will get lost.
-   *)
-  remember (C0 with_locals = ts with_return = None) as C.
-  remember ([] --> rt) as progtype.
-  induction HVIS as [ | ? ? ? ? ? ? ? HVIS' IHHVIS' HVI__N ]; (* [eqn:H] failed? *)
-    introv HSC;
-    simpl in HSC;
-    remember {| A_locals := vals; A_module := mi |} as F;
+  (* valid_config *)
+  inverts keep HVC as HSok HVT.
+    (* valid_store *)
+    (* valid_thread *)
+    inverts keep HVT as HVA HVAIS.
+      (* valid_frame *)
+      inverts keep HVA as HVMI HVV.
+        (* valid_moduleinst *)
+        (* valid_value *)
+      (* valid_admin_instrs *)
+
+  gen S' T'.
+  dependent induction HVAIS; 
+    introv HSC; simpl in HSC;
     destruct T' as [F' ainstrs'].
 
-  - (* VIS_empty *)
+  - (* VAIS_empty *)
     exfalso.
-    apply (S_F_ϵ_is_normal_form S F S' F'). 
+    eapply (S_F_ϵ_is_normal_form S _ S' F'). 
     exists ainstrs'...
 
-  - (* VIS_snoc *)
-    remember (S, F, ↑ (instrs ++ [instr__N])) as SF.
-    remember (S', F', ainstrs') as SF'.
-    induction HSC as [ ? ? ? ? HSS | ];
-      inverts Heqprogtype;
-      inverts HeqSF;
-      inverts HeqSF'.
-      
+  - (* remember {| A_locals := vals; A_module := mi |} as F; *)
+    (* VAIS_snoc:
+
+      [HVAIS : S0,C1 ⊢a* ainstrs ∈ ts1 --> (ts0 ++ ts2)]
+      [HVAI__N : S0,C1 ⊢a  ainstr__N ∈ ts2 --> ts3]                      (* H *)
+      [HSC   : (S, F, (ainstrs ++ [ainstr__N])) ↪ (S', F', ainstrs')]
+       ------------------------------------------------------------
+      [⊢c (S', (F', ainstrs')) ∈ rt /\ ⊢S S ⪯ S']
+
+     *)
+    dependent induction HSC.
     + (* SC_simple *)
-      inverts keep HVI__N. (* invert typing [instrN] *)
+      split. 
+      ++ (* Preserve Type *)
+          constructor; try apply HSok.
+          econstructor; try apply HVA...
+          eapply preservation_SC_simple...
 
-      ++ (* VI_const *)
-         exfalso.
-         simpl in HSS.
-         apply (snoc_val_is_normal_form instrs val).
-         exists ainstrs'...
+      ++ (* Preserve Store *) (* [⊢S S ⪯ S] *)
+         apply (extend_store_refl _ HSok). 
 
-      ++ (* VI_unop *)
-         inverts HSS as. (* invert [step_simple] relation *)
-
-        +++ (* [SS_unop__some] *)
-            introv Heval_unop Heq.
-
-            replace ([Plain (Const val1); Plain (Unop op0)])
-               with (↑([Const val1] ++ [Unop op0])) in Heq.
-            apply lift_up_eq in Heq.
-            apply app_snoc_destruct in Heq.
-            inverts Heq as Heqop; inverts Heqop.
-
-            split.
-            ++++ constructor.
-                 assumption.
-                 subst. (* rewrite <- TEMP. *)
-                 econstructor. apply HVA.
-                 constructor. replace ([Const val]) with ([] ++ [Const val]).
-                 eapply VIS_snoc.
-                 apply drop_singleton_typing in HVIS'.
-                 inverts HVIS'.
-                 skip. (* eapply VIS_empty. *)
-                 apply VI_const.
-                 apply (eval_unop_inv _ val1)...
-                 reflexivity.
-                 trivial.
-            ++++ skip.
-            ++++ simpl. reflexivity.
-
-        +++ (* [SS_unop__none] *)
-            skip.
-           
-        +++ (* contradiction *)
-            intros.
-            replace ([Plain (Const c1); Plain (Const c2); Plain (Binop op0)])
-               with (↑([Const c1; Const c2] ++ [Binop op0])) in H.
-            apply lift_up_eq in H.
-            false H.
-            apply unsnoc_neq in H...
-            replace (unsnoc ([Const c1; Const c2] ++ [Binop op0])) with (Some (Binop op0)). 
-            replace (unsnoc (instrs ++ [Unop op])) with (Some (Unop op)). 
-            unfold not; intros. false H1.
-            skip. (* eapply (unsnoc_snoc_app instrs (Unop op)).  *)
-            skip.  (* eapply unsnoc_snoc_app. *)
-            reflexivity.
-
-        +++ (* contradiction *) skip.
-        +++ (* contradiction *) skip.
-        +++ (* contradiction *) skip.
-
-      (* should be similar with VI_unop,
-         will polish the proof and extract them as lemma. *)
-      ++ (* VI_binop *)
-         admit.
-      ++ (* VI_testop *)
-         admit.
-      ++ (* VI_relop *)
-         admit.
-                                        
-    + (* SC_E *)
+    + (* SC_E *) (* Harder *)
       admit.
+
+Admitted.
+
   
+   
+
